%This is a LaTeX template for homework assignments
\documentclass{article}

\usepackage[utf8]{inputenc}
\usepackage{amsmath}
\usepackage{amssymb}
\usepackage{graphicx}
\usepackage{enumitem}

\begin{document}

%\title{EMET1001: ASSIGNMENT WEEK 2}
%\author{ZEMING WANG - U6114134}


%\maketitle
%\vspace{1in}

%TUTOR: LONG

\thispagestyle{empty}

\begin{center}
\huge
\vspace*{1.0in} EMET1001 
\\\vspace{0.5in} ASSIGNMENT 8
\normalsize
\\\vspace{0.5in} \textsc{By}
\\\vspace{0.1in} \textsc{Zeming Wang}
\\\vspace{0.1in} \textsc{u6114134}
\normalsize
\\\vspace{0.5in} \textsc{Tutorial: Thur. 2-3 pm}
\\\vspace{0.1in} \textsc{Tutor: Long}
\normalsize
\\\vspace{0.5in} \textsc{Due: Sept. 27, 2016}
\end{center}

\newpage
\setcounter{page}{1}

\begin{enumerate}
    
    \item[3.] Let $f(x,y,z) = \sqrt{x^2 + y^2 + z^2}$. Calculate $f(3,4,0)$, $f(-2,1,3)$, and $f(tx,ty,tz)$ for $t \geq 0$. \\
    
    Solution:
    $$ f(3,4,0) = \sqrt{3^2 + 4^2 +0^2} = 5 $$
    $$ f(-2,1,3) = \sqrt{(-2)^2 + 1^2 + 3^3} = \sqrt{14} $$
    $$ f(tx, ty, tz) = \sqrt{(tx)^2 + (ty)^2 + (tz)^2} = t\sqrt{x^2+y^2+z^2} $$
    
    \item[6.] For which pairs of numbers $(x,y)$ are the functions given by the following formulas defined?
    
        \begin{enumerate}
            \item[(a)] $3xy^3 - 45x^4 - 3y$ \\
            
            The function is well-defined for all real numbers, so $(x,y) \in \mathbb{R}^2$.\\
            
            \item[(b)] $\sqrt{1 - xy}$ \\
            
            $1-xy$ must be non-negative, i.e. $ 1 - xy \geq 0 \Leftrightarrow xy \leq 1$. Therefore, $(x,y) \in \{(x,y): xy \leq 1\}$.\\
            
            \item[(c)] $\ln{(2 - (x^2 + y^2))}$ \\
            
            The domain of $\ln{}$ function contains only positive numbers, which implies $2 - (x^2 + y^2) > 0 \Leftrightarrow x^2 + y^2 < 2$. Therefore, $(x,y) \in \{ (x,y): x^2 + y^2 < 2 \}$.
            
        \end{enumerate}
    
    \item[9. ] Let $f$ be defined for all $(x,y)$ by $f(x,y)=(x-2)^2(y+3)^2$.
        \begin{enumerate}
            \item[(a)] Calculate $f(0, 0)$, $f(-2, -3)$, and $f(a + 2, b - 3)$. \\
            
            Solution: 
            $$ f(0,0) = (0-2)^2(0+3)^2 = 36 $$
            $$ f(-2,-3) = (-2-2)^2(-3+3)^2 = 0 $$
            $$ f(a+2,b-3) = (a+2-2)^2(b-3+3)^2 = a^2b^2 $$
            
            \item[(b)] Find $f_x$ and $f_y$. \\
            
            Solution:
            $$ f_x = 2(x-2)(y+3)^2 $$
            $$ f_y = 2(x-2)^2(y+3) $$

        \end{enumerate}
        
    \item[11. ] For each $c \neq 0$,verify that $x-y = c$ is a level curve for $$ F(x,y) = \ln{(x^2 - 2xy + y^2)} + e^{2x-2y} $$ 
    
    Solution: Substitute $x-y=c$ into $F$, we have:
    $$ F(x,y) = \ln{(x-y)^2} + e^{2(x-y)} = \ln{c^2} + e^{2c} $$
    which is a constant. That means, all $(x,y)$ that satisfy $x-y = c$ yield the same value from $F(x,y)$. Therefore, $x-y=c$ is a level curve for $F(x,y)$ for all $c \neq 0$.
    
    \item[13. ] Find the partial elasticities of z w.r.t. $x$ and $y$ in the following cases.
        \begin{enumerate}
            \item[(a)] $z = x^3y^{-4}$
            $$ E_x = \frac{\partial z}{\partial x}\frac{x}{z} = 3x^2y^{-4} \cdot \frac{x}{x^3y^{-4}} = 3 $$
            $$ E_y = \frac{\partial z}{\partial y}\frac{y}{z} = -4x^3y^{-5} \cdot \frac{y}{x^3y^{-4}} = -4 $$
            
            \item[(b)] $z =\ln{(x^2 + y^2)}$
            $$ E_x = \frac{\partial z}{\partial x}\frac{x}{z} = \frac{2x}{x^2+y^2} \cdot \frac{x}{\ln{(x^2+y^2)}} = \frac{2x^2}{(x^2+y^2)\ln{(x^2+y^2)}} $$
            $$ E_y = \frac{\partial z}{\partial y}\frac{y}{z} = \frac{2y}{x^2+y^2} \cdot \frac{y}{\ln{(x^2+y^2)}} = \frac{2y^2}{(x^2+y^2)\ln{(x^2+y^2)}} $$
            
            \item[(c)] $z = e^{x+y}$
            $$ E_x = \frac{\partial z}{\partial x}\frac{x}{z} = e^{x+y}\frac{x}{e^{x+y}} = x $$
            $$ E_y = \frac{\partial z}{\partial y}\frac{y}{z} = e^{x+y}\frac{y}{e^{x+y}} = y $$
            
            \item[(d)] $z = \sqrt{x^2 + y^2}$
            $$ E_x = \frac{\partial z}{\partial x}\frac{x}{z} = \frac{2x}{2\sqrt{x^2+y^2}} \cdot \frac{x}{\sqrt{x^2+y^2}} = \frac{x^2}{x^2+y^2} $$
            $$ E_y = \frac{\partial z}{\partial y}\frac{y}{z} = \frac{2y}{2\sqrt{x^2+y^2}} \cdot \frac{y}{\sqrt{x^2+y^2}} = \frac{y^2}{x^2+y^2} $$
            
        \end{enumerate}
        
\end{enumerate}

\end{document}