%This is a LaTeX template for homework assignments
\documentclass{article}

\usepackage[utf8]{inputenc}
\usepackage{amsmath}
\usepackage{amssymb}
\usepackage{graphicx}
\usepackage{enumitem}

\begin{document}

%\title{EMET1001: ASSIGNMENT WEEK 2}
%\author{ZEMING WANG - U6114134}


%\maketitle
%\vspace{1in}

%TUTOR: LONG

\thispagestyle{empty}

\begin{center}
\huge
\vspace*{1.0in} EMET1001 
\\\vspace{0.5in} ASSIGNMENT 11
\normalsize
\\\vspace{0.5in} \textsc{By}
\\\vspace{0.1in} \textsc{Zeming Wang}
\\\vspace{0.1in} \textsc{u6114134}
\normalsize
\\\vspace{0.5in} \textsc{Tutorial: Thur. 2-3 pm}
\\\vspace{0.1in} \textsc{Tutor: Long}
\normalsize
\\\vspace{0.5in} \textsc{Due: Oct. 17, 2016}
\end{center}

\newpage
\setcounter{page}{1}


\begin{enumerate}
    \item[1. ] Construct the two matrices $\mathbf{A} = (a_{ij})_{2 \times 3}$, where
        \begin{enumerate}
            \item[(a)] $a_{ij} = i + j$
            $$ \mathbf{A} = \begin{pmatrix}2 &3 &4 \\3 &4 &5 \end{pmatrix} $$
            \item[(b)] $a_{ij} = (-1)^{i+j}$
            $$ \mathbf{A} = \begin{pmatrix}1 &-1 &1 \\-1 &1 &-1 \end{pmatrix} $$
        \end{enumerate}
        
    \item[2. ] Using the matrices
    $$ \mathbf{A} = \begin{pmatrix}2 &0\\-1 &1\end{pmatrix}\ 
       \mathbf{B} = \begin{pmatrix}-1 &2\\1 &-1\end{pmatrix}\
       \mathbf{C} = \begin{pmatrix}2 &3\\1 &4\end{pmatrix}\
       \mathbf{D} = \begin{pmatrix}1 &1 &1\\1 &3 &4\end{pmatrix}\
    $$
    calculate (where possible)
        \begin{enumerate}
            \item[(a)] $\mathbf{A} - \mathbf{B}$
            \begin{align*}
                \mathbf{A} - \mathbf{B} 
                =  \begin{pmatrix}2 &0\\-1 &1\end{pmatrix} 
                - \begin{pmatrix}-1 &2\\1 &-1\end{pmatrix} 
                = \begin{pmatrix}3 &-2\\-2 &2\end{pmatrix}
            \end{align*}
            
            \item[(b)] $\mathbf{A} + \mathbf{B} - 2\mathbf{C}$
            \begin{align*}
                \mathbf{A} + \mathbf{B} - 2\mathbf{C} 
                &= \begin{pmatrix}2 &0\\-1 &1\end{pmatrix}
                 + \begin{pmatrix}-1 &2\\1 &-1\end{pmatrix}
                 - 2\begin{pmatrix}2 &3\\1 &4\end{pmatrix} \\
                & \\
                &= \begin{pmatrix}1 &2\\0 &0\end{pmatrix}
                 - \begin{pmatrix}4 &6\\2 &8\end{pmatrix} 
                 = \begin{pmatrix}-3 &-4\\-2 &-8\end{pmatrix} 
            \end{align*}

            \item[(c)] $\mathbf{A}\mathbf{B}$
            \begin{align*}
                \mathbf{A}\mathbf{B}
                = \begin{pmatrix}2 &0\\-1 &1\end{pmatrix}
                  \begin{pmatrix}-1 &2\\1 &-1\end{pmatrix}
                = \begin{pmatrix}-2 &4\\2 &-3\end{pmatrix}
            \end{align*}
            
            \item[(d)] $\mathbf{C}(\mathbf{A}\mathbf{B})$
            \begin{align*}
                \mathbf{C}(\mathbf{A}\mathbf{B})
                = \begin{pmatrix}2 &3\\1 &4\end{pmatrix}
                  \begin{pmatrix}-2 &4\\2 &-3\end{pmatrix}
                = \begin{pmatrix}2 &-1\\6 &-8\end{pmatrix}
            \end{align*}
            
            \item[(e)] $\mathbf{A}\mathbf{D}$
            \begin{align*}
                \mathbf{A}\mathbf{D}
                = \begin{pmatrix}2 &0\\-1 &1\end{pmatrix}
                  \begin{pmatrix}1 &1 &1\\1 &3 &4\end{pmatrix}
                = \begin{pmatrix}2 &2 &2\\0 &2 &3\end{pmatrix}
            \end{align*}
            \item[(f)] $\mathbf{D}\mathbf{C}$
            $$ \mathbf{D}\mathbf{C}\ \textrm{is not possible.}$$
            
        \end{enumerate}

    \item[3. ] Using the matrices in Problem 2, compute (where possible)
    % $$ \mathbf{A} = \begin{pmatrix}2 &0\\-1 &1\end{pmatrix}\ 
    %    \mathbf{B} = \begin{pmatrix}-1 &2\\1 &-1\end{pmatrix}\
    %    \mathbf{C} = \begin{pmatrix}2 &3\\1 &4\end{pmatrix}\
    %    \mathbf{D} = \begin{pmatrix}1 &1 &1\\1 &3 &4\end{pmatrix}\
    % $$
        \begin{enumerate}
            \item[(a)] $2\mathbf{A} - 3\mathbf{B}$
            \begin{align*}
                2\mathbf{A} - 3\mathbf{B}
                = 2\begin{pmatrix}2 &0\\-1 &1\end{pmatrix}
                - 3\begin{pmatrix}-1 &2\\1 &-1\end{pmatrix}
                = \begin{pmatrix}4 &0\\-2 &2\end{pmatrix}
                - \begin{pmatrix}-3 &6\\3 &-3\end{pmatrix}
                = \begin{pmatrix}7 &-6\\-5 &5\end{pmatrix}
            \end{align*}
            
            \item[(b)] $(\mathbf{A} - \mathbf{B})'$
            \begin{align*}
                (\mathbf{A} - \mathbf{B})' 
                =  \Bigg( \begin{pmatrix}2 &0\\-1 &1\end{pmatrix} 
                - \begin{pmatrix}-1 &2\\1 &-1\end{pmatrix} \Bigg)'
                = \begin{pmatrix}3 &-2\\-2 &2\end{pmatrix}'
                = \begin{pmatrix}3 &-2\\-2 &2\end{pmatrix}
            \end{align*}
            
            \item[(c)] $(\mathbf{C}'\mathbf{A}')\mathbf{B}'$
            \begin{align*}
                (\mathbf{C}'\mathbf{A}')\mathbf{B}'
                = \left( \begin{pmatrix}2 &1\\3 &4\end{pmatrix} 
                  \begin{pmatrix}2 &-1\\0 &1\end{pmatrix} \right)
                  \begin{pmatrix}-1 &1\\2 &-1\end{pmatrix}
                = \begin{pmatrix}4 &-1\\6 &1\end{pmatrix}
                  \begin{pmatrix}-1 &1\\2 &-1\end{pmatrix}
                = \begin{pmatrix}-6 &5\\-4 &5\end{pmatrix}
            \end{align*}
            
            \item[(d)] $\mathbf{C}'(\mathbf{A}'\mathbf{B}')$
            \begin{align*}
                \mathbf{C}'(\mathbf{A}'\mathbf{B}')
                = \begin{pmatrix}2 &1\\3 &4\end{pmatrix} 
                  \left( \begin{pmatrix}2 &-1\\0 &1\end{pmatrix}
                  \begin{pmatrix}-1 &1\\2 &-1\end{pmatrix} \right)
                = \begin{pmatrix}2 &1\\3 &4\end{pmatrix} 
                  \begin{pmatrix}-4 &3\\2 &-1\end{pmatrix}
                = \begin{pmatrix}-6 &5\\-4 &5\end{pmatrix}
            \end{align*}
            
            \item[(e)] $\mathbf{D}'\mathbf{D}'$
            $$ \mathbf{D}'\ \textrm{is not square matrix. The multiplication is not possible. }$$
            
            \item[(f)] $\mathbf{D}'\mathbf{D}$
            \begin{equation*}
                \mathbf{D}'\mathbf{D}
                = \begin{pmatrix}1 &1\\1 &3\\1 &4\end{pmatrix}
                  \begin{pmatrix}1 &1 &1\\1 &3 &4\end{pmatrix}
                = \begin{pmatrix}2 &4 &5\\4 &10 &13\\5 &13 &17\end{pmatrix}
            \end{equation*}
        \end{enumerate}
        
    \item[4. ] Write the following systems of equations in matrix notation:
        \begin{enumerate}
            \item[(a)]
            \begin{align*}
                2x_1 - 5x_2 &= 3 \\
                5x_1 + 8x_2 &= 5 \\
            \end{align*}
            Matrix form:
            \begin{equation*}
                \begin{pmatrix}2 &-5\\5 &8\end{pmatrix}
                \begin{pmatrix}x_1\\x_2\end{pmatrix}   
                = \begin{pmatrix}3\\5\end{pmatrix}   
            \end{equation*}
            
            \item[(b)]
            \begin{align*}
                x + y + z + t    &= a \\
                x + 3y + 2z + 4t &= b \\
                x + 4y + 8z      &= c \\
                2x + z - t       &= d \\
            \end{align*}
            Matrix form:
            \begin{equation*}
                \begin{pmatrix}
                    1 &1 &1 &1\\
                    1 &3 &2 &4\\
                    1 &4 &8 &0\\
                    2 &0 &1 &-1\\
                \end{pmatrix}
                \begin{pmatrix}x\\y\\z\\t\end{pmatrix}
                = \begin{pmatrix}a\\b\\c\\d\end{pmatrix}
            \end{equation*}
            
            \item[(c)] 
            \begin{align*}
                ax + y + (a + 1)z &= b_1 \\
                x + 2y + z        &= b_2 \\
                3x + 4y + 7z      &= b_3 \\
            \end{align*}
            Matrix form:
            \begin{equation*}
                \begin{pmatrix}
                    a &1 &a+1 \\
                    1 &2 &1   \\
                    3 &4 &7   \\
                \end{pmatrix}
                \begin{pmatrix}x\\y\\z\end{pmatrix}
                = \begin{pmatrix}b_1\\b_2\\b_3\end{pmatrix}
            \end{equation*}
            
        \end{enumerate}
        
    \item[10. ] Let $\mathbf{a} = (-1,5,3)$, $\mathbf{b} = (1,1,-3)$, and $\mathbf{c}=(-1,2,8)$. Compute $\|a\|$, $\|b\|$, and $\|c\|$. Then verify that the Cauchy-Schwarz inequality holds for $\mathbf{a}$ and $\mathbf{b}$. \\
    
    \textbf{Solution}: 
    \begin{align*}
        \|\mathbf{a}\| &= \sqrt{(-1)^2 + 5^2 + 3^2} = \sqrt{35} \\
        \|\mathbf{b}\| &= \sqrt{1^2 + 1^2 + (-3)^2} = \sqrt{11} \\
        \|\mathbf{a}\| &= \sqrt{(-1)^2 + 2^2 + 8^2} = \sqrt{69} \\
    \end{align*}
    To verify the Cauchy-Schwarz inequality, compute:
    $$ | \mathbf{a} \cdot \mathbf{b} | = | (-1) \times 1 + 5 \times 1 + 3 \times (-3) | = 5 $$
    $$ \|\mathbf{a}\| \cdot \|\mathbf{b}\| = \sqrt{35} \cdot \sqrt{11} = \sqrt{385} \approx 19.62 $$
    Therefore, the Cauchy-Schwarz inequality holds:
    $$ | \mathbf{a} \cdot \mathbf{b} | \leq \|\mathbf{a}\| \cdot \|\mathbf{b}\| $$
    
\end{enumerate}

\end{document}